Progress on log

composition/log.fst
@@ -15,17 +15,6 @@ let rec unique_s l =
   |[] -> true
   |(id,m)::xs -> not (mem_id_s id xs) && unique_s xs
 
-val pos : id:(nat * string) -> l:list (nat * string) {mem id l /\ unique_s l} -> Tot nat
-let rec pos id l =
-  match l with
-  |id1::xs -> if id = id1 then 0 else 1 + pos id xs
-
-val ord : id:(nat * string)
-        -> id1:(nat * string) {fst id <> fst id1} 
-        -> l:list (nat * string){mem id l /\ mem id1 l /\ unique_s l} 
-        -> Tot (b:bool {b = true <==> pos id l < pos id1 l})
-let ord id id1 l = pos id l < pos id1 l 
-
 val total_order : l:list (nat * string) {unique_s l}
                 -> Tot (b:bool)
 let rec total_order l =
@@ -33,6 +22,20 @@ let rec total_order l =
   |[] -> true
   |[(id,m)] -> true
   |(id, m)::(id1, m1)::xs -> id > id1 && total_order ((id1, m1)::xs)
+
+  val pos : id:(nat * string) -> l:list (nat * string) {mem id l /\ unique_s l /\ total_order l} -> Tot nat
+  let rec pos id l =
+    match l with
+    |id1::xs -> if id = id1 then 0 else 1 + pos id xs
+
+
+val ord : id:(nat * string)
+          -> id1:(nat * string)
+          -> l:list (nat * string)
+          -> Pure bool
+            (requires fst id <> fst id1 /\ mem id l /\ mem id1 l /\ unique_s l /\ total_order l)
+            (ensures (fun b -> b = true <==> pos id l < pos id1 l))
+let ord id id1 l = pos id l < pos id1 l 
 
 type s = l: list (nat (*id*) * string (*message*)) {unique_s l /\ total_order l}
 
@@ -58,6 +61,16 @@ val app_op : s1:s
              (ensures (fun r -> (forall e. mem e r <==> mem e s1 \/ e = (get_id op1, get_msg op1))))
 let app_op s1 (id, (Append m)) = (id, m)::s1
 
+val filter_uni : f:((nat * string) -> bool)
+                 -> l:list (nat * string) 
+                 -> Lemma (requires (unique_s l /\ total_order l))
+                          (ensures (unique_s (filter f l) /\ total_order (filter f l)))
+                          [SMTPat (filter f l)]
+let rec filter_uni f l = admit();
+    match l with
+    |[] -> ()
+    |x::xs -> filter_uni f xs
+
 (*)instance log : datatype s op = {
   Library.app_op = app_op
 }*)
@@ -70,7 +83,15 @@ val sim : tr:ae op
                                       mem (fst e, (Append (snd e))) tr.l /\ mem (fst e1, (Append (snd e1))) tr.l /\
                              fst e <> fst e1 /\ fst e > fst e1 /\ tr.vis (fst e1, (Append (snd e1))) (fst e, (Append (snd e))))})
 
-let sim tr s1 = admit()
+#set-options "--z3rlimit 1000000"
+let sim tr s1 =
+  forallb (fun e -> mem (fst e, (Append (snd e))) tr.l) s1 &&
+  forallb (fun e -> mem (get_id e, get_msg e) s1) tr.l &&
+  forallb (fun e -> (forallb (fun e1 ->  mem (fst e, (Append (snd e))) tr.l && mem (fst e1, (Append (snd e1))) tr.l &&
+              fst e <> fst e1 && fst e > fst e1 && tr.vis (fst e1, (Append (snd e1))) (fst e, (Append (snd e))))
+  (filter (fun e1 -> mem e1 s1 && mem e s1 && fst e <> fst e1 && fst e > fst e1 && ord e e1 s1) s1))) s1 &&
+  forallb (fun e -> (forallb (fun e1 -> mem (get_id e, get_msg e) s1 && mem (get_id e1, get_msg e1) s1 && get_id e <> get_id e1 && get_id e > get_id e1 && ord (get_id e, get_msg e) (get_id e1, get_msg e1) s1)
+          (filter (fun e1 -> get_id e <> get_id e1 && get_id e > get_id e1 && tr.vis e1 e) tr.l))) tr.l
 
 val prop_oper : tr:ae op
               -> st:s
@@ -80,7 +101,7 @@ val prop_oper : tr:ae op
                       (ensures (sim (append tr op) (app_op st op)))
 let prop_oper tr st op = ()
 
-val convergence1 : tr:ae op
+val convergence : tr:ae op
                     -> a:s
                     -> b:s
                     -> Lemma (requires (sim tr a /\ sim tr b))
@@ -88,75 +109,17 @@ val convergence1 : tr:ae op
                                      (forall e e1. mem e a /\ mem e1 a /\ fst e <> fst e1 /\ ord e e1 a /\ fst e > fst e1 <==> 
                                               mem e b /\ mem e1 b /\ fst e <> fst e1 /\ ord e e1 b /\ fst e > fst e1))
                             [SMTPat (sim tr a /\ sim tr b)]
-let convergence1 tr a b = ()
-
-  val remove_st : ele:(nat * string) -> a:s
-                -> Pure s
-                  (requires (mem ele a))
-                  (ensures (fun r -> (forall e. mem e r <==> mem e a /\ e <> ele) /\
-                                  (forall id. mem_id_s id r <==> mem_id_s id a /\ id <> fst ele) /\
-                                  (forall e e1. mem e r /\ mem e1 r /\ fst e <> fst e1 /\ ord e e1 r /\ fst e > fst e1 <==>
-                                           mem e a /\ mem e1 a /\ fst e <> fst e1 /\ e <> ele /\ e1 <> ele /\ fst e > fst e1 /\ ord e e1 a) /\ List.Tot.length r = List.Tot.length a - 1))
-  #set-options "--z3rlimit 10000"
-  let rec remove_st ele a =
-    match a with
-    |ele1::xs -> if ele = ele1 then xs 
-                  else ((assume (forall e. mem e xs ==> fst ele1 > fst e)); ele1::(remove_st ele xs))
-
-val lem_len : a:s -> b:s
-                     -> Lemma (requires (forall id. mem_id_s id a <==> mem_id_s id b) /\ (forall e. mem e a <==> mem e b) /\
-                                      (forall e e1. mem e a /\ mem e1 a /\ fst e <> fst e1 /\ ord e e1 a /\ fst e > fst e1 <==> 
-                                               mem e b /\ mem e1 b /\ fst e <> fst e1 /\ ord e e1 b /\ fst e > fst e1))
-                           (ensures (List.Tot.length a = List.Tot.length b))
-let rec lem_len a b = 
-  match a,b with
-  |[],[] -> ()
-  |x::xs, _ -> lem_len xs (remove_st x b)
-
-val lem_same : a:s -> b:s
-             -> Lemma (requires (forall id. mem_id_s id a <==> mem_id_s id b) /\ (forall e. mem e a <==> mem e b) /\
-                                  (List.Tot.length a = List.Tot.length b) /\
-                                  (forall e e1. mem e a /\ mem e1 a /\ fst e <> fst e1 /\ fst e > fst e1 /\ ord e e1 a <==> 
-                                           mem e b /\ mem e1 b /\ fst e <> fst e1 /\ fst e > fst e1 /\ ord e e1 b))
-                       (ensures (forall e. mem e a /\ mem e b ==> pos e a = pos e b))
-
-#set-options "--z3rlimit 10000000"
-let rec lem_same a b = admit();
-  match a, b with
-  |[],[] -> ()
-  |x::xs, _ -> lem_same xs (remove_st x b)
-
-val lem_same1 : a:s -> b:s
-               -> Lemma (requires (forall id. mem_id_s id a <==> mem_id_s id b) /\ (forall e. mem e a <==> mem e b) /\
-                                    (List.Tot.length a = List.Tot.length b) /\
-                                    (forall e e1. mem e a /\ mem e1 a /\ fst e <> fst e1 /\ fst e > fst e1 /\ ord e e1 a <==> 
-                                             mem e b /\ mem e1 b /\ fst e <> fst e1 /\ fst e > fst e1 /\ ord e e1 b) /\
-                                             (forall e. mem e a /\ mem e b ==> pos e a = pos e b))
-                                 (ensures a = b)
-
-#set-options "--z3rlimit 10000000"
-let rec lem_same1 a b =
-    match a, b with
-    |[],[] -> ()
-    |x::xs, _ -> lem_same1 xs (remove_st x b)
-    
-val convergence : tr:ae op
-                  -> a:s
-                  -> b:s
-                  -> Lemma (requires (sim tr a /\ sim tr b))
-                          (ensures a = b)
-                          [SMTPat (sim tr a /\ sim tr b)]
-let convergence tr a b = 
-  convergence1 tr a b;
-  lem_len a b;
-  lem_same a b; 
-  lem_same1 a b;
-  ()
+let convergence tr a b = ()
 
 val merge1 : l:s -> a:s -> b:s
            -> Pure s
              (requires true)
-             (ensures (fun r -> (forall e. mem e r <==> mem e a \/ mem e b)))
+             (ensures (fun r -> (forall e. mem e r <==> mem e a \/ mem e b) /\
+                             (forall e e1. mem e r /\ mem e1 r /\ fst e <> fst e1 /\ fst e > fst e1 /\ ord e e1 r <==>
+                                     (mem e a /\ mem e1 a /\ fst e <> fst e1 /\ fst e > fst e1 /\ ord e e1 a) \/
+                                     (mem e b /\ mem e1 b /\ fst e <> fst e1 /\ fst e > fst e1 /\ ord e e1 b) \/
+                                     (mem e a /\ mem e1 b /\ fst e <> fst e1 /\ fst e > fst e1) \/
+                                     (mem e b /\ mem e1 a /\ fst e <> fst e1 /\ fst e > fst e1))))
 let merge1 l a b = admit()
 
 val merge : ltr:ae op
@@ -190,8 +153,23 @@ val prop_merge : ltr:ae op
                                  (forall e e1. mem e ltr.l /\ mem e1 btr.l ==> get_id e < get_id e1) /\
                                  (sim ltr l /\ sim (union ltr atr) a /\ sim (union ltr btr) b))
                        (ensures (sim (absmerge ltr atr btr) (merge ltr l atr a btr b)))
+
 #set-options "--z3rlimit 10000000"
-let prop_merge ltr l atr a btr b = ()
+let prop_merge ltr l atr a btr b = 
+    assert (forall e. mem e (merge ltr l atr a btr b) <==> mem (fst e, (Append (snd e))) (absmerge ltr atr btr).l);
+    assume (forall e e1. mem e (merge ltr l atr a btr b) /\ mem e1 (merge ltr l atr a btr b) /\ fst e <> fst e1 /\ 
+                fst e > fst e1 /\ ord e e1 (merge ltr l atr a btr b) ==>
+                mem (fst e, (Append (snd e))) (absmerge ltr atr btr).l /\ 
+                mem (fst e1, (Append (snd e1))) (absmerge ltr atr btr).l /\
+                fst e <> fst e1 /\ fst e > fst e1 /\ 
+                (absmerge ltr atr btr).vis (fst e1, (Append (snd e1))) (fst e, (Append (snd e))));
+    assert (forall e e1. mem e (absmerge ltr atr btr).l /\ mem e1 (absmerge ltr atr btr).l /\ get_id e <> get_id e1 /\ 
+                    get_id e > get_id e1 /\ (absmerge ltr atr btr).vis e1 e ==> 
+                      mem (get_id e, get_msg e) (merge ltr l atr a btr b) /\ 
+                        mem (get_id e1, get_msg e1) (merge ltr l atr a btr b) /\
+             get_id e <> get_id e1 /\ get_id e > get_id e1 /\ 
+             ord (get_id e, get_msg e) (get_id e1, get_msg e1) (merge ltr l atr a btr b));
+             ()
 
 
 
